Get started on 101, but missing the material from Lean master

HumanEvalLean/HumanEval101.lean
@@ -1,7 +1,42 @@
 module
 
-def words_string : Unit :=
-  ()
+def wordsString (s : String) : Array String :=
+  s.split (fun c => c = ',' ∨ c = ' ')
+    |>.filter (!·.isEmpty)
+    |>.toStringArray
+
+example : wordsString "Hi, my name is John" = #["Hi", "my", "name", "is", "John"] := by native_decide
+example : wordsString "One, two, three, four, five, six" = #["One", "two", "three", "four", "five", "six"] := by native_decide
+example : wordsString "Hi, my name" = #["Hi", "my", "name"] := by native_decide
+example : wordsString "One,, two, three, four, five, six," = #["One", "two", "three", "four", "five", "six"] := by native_decide
+example : wordsString "" = #[] := by native_decide
+example : wordsString "ahmed     , gamal" = #["ahmed", "gamal"] := by native_decide
+
+theorem wordsString_eq (s : String) : wordsString s =
+    (s.split (fun c => c = ',' ∨ c = ' ')
+      |>.toList
+      |>.map String.Slice.copy
+      |>.filter (!·.isEmpty)
+      |>.toArray) := by
+  simp [← Array.toList_inj, wordsString, List.filter_map]
+  congr
+  · sorry -- will be easy in next nightly
+  · ext; simp [String.Slice.isEmpty_copy]
+
+
+theorem wordsString_empty : wordsString "" = #[] := by
+  rw [wordsString_eq]
+  sorry
+
+theorem wordsString_singleton_append_of_or (s : String) (c : Char) (hc : c = ',' ∨ c = ' ') :
+    wordsString (String.singleton c ++ s) = wordsString s := by
+  sorry
+
+theorem wordsString_append_append (s t : String) (hs : ',' ∉ s.toList) (hs' : ' ' ∉ s.toList)
+    (c : Char) (hc : c = ',' ∨ c = ' ') :
+    wordsString (s ++ String.singleton c ++ t) = #[s] ++ wordsString t :=
+  sorry
+
 
 /-!
 ## Prompt
@@ -12,7 +47,7 @@ def words_string(s):
     """
     You will be given a string of words separated by commas or spaces. Your task is
     to split the string into words and return an array of the words.
-    
+
     For example:
     words_string("Hi, my name is John") == ["Hi", "my", "name", "is", "John"]
     words_string("One, two, three, four, five, six") == ["One", "two", "three", "four", "five", "six"]
